asms/riscv64/RiscV_Instructions.thy
@@ -17,10 +17,12 @@ begin
 
 subsubsection \<open>ADDI\<close>
 
+abbreviation \<open>addi w rd rs1 imm \<equiv> \<lparr> addr = w, size = (4 \<Colon> 64), code = [rd := (rs1 :\<^sub>t imm\<langle>64\<rangle>) + (imm \<Colon> 64)] \<rparr>\<close>
+
 lemma step_addi:
-  assumes decode_addi: \<open>\<And>\<Delta> var. (\<Delta>, (address \<Colon> 64), var) \<mapsto>\<^sub>b\<^sub>i\<^sub>l \<lparr> addr = (address \<Colon> 64), size = (4 \<Colon> 64), code = [rd := (rs1 :\<^sub>t imm\<langle>64\<rangle>) + (imm \<Colon> 64)] \<rparr>\<close>
+  assumes decode_addi: \<open>\<And>\<Delta> var. (\<Delta>, w, var) \<mapsto>\<^sub>b\<^sub>i\<^sub>l addi w rd rs1 imm\<close>
       and \<open>(rs1 :\<^sub>t imm\<langle>64\<rangle>, val \<Colon> 64) \<in>\<^sub>\<Delta> \<Delta>\<close>
-    shows \<open>(\<Delta>, address \<Colon> 64, var) \<leadsto>\<^sub>b\<^sub>i\<^sub>l (\<Delta>(rd \<mapsto> (val \<Colon> 64) +\<^sub>b\<^sub>v (imm \<Colon> 64)), (address \<Colon> 64) +\<^sub>b\<^sub>v (4 \<Colon> 64), var)\<close>
+    shows \<open>(\<Delta>, w, var) \<leadsto>\<^sub>b\<^sub>i\<^sub>l (\<Delta>(rd \<mapsto> (val \<Colon> 64) +\<^sub>b\<^sub>v (imm \<Colon> 64)), w +\<^sub>b\<^sub>v (4 \<Colon> 64), var)\<close>
   apply (insert assms(2-))
   by (solve_progI decoder: decode_addi)
 
@@ -30,19 +32,23 @@ subsubsection \<open>SEXT.W\<close>
 
 text \<open>Pseudonym for ADDIW when imm = 0.\<close>
 
+abbreviation \<open>sextw w rd rs1 \<equiv> \<lparr> addr = w, size = (4 \<Colon> 64), code = [rd := (extend:64[low:32[(rs1 :\<^sub>t imm\<langle>64\<rangle>)]])] \<rparr>\<close>
+
 lemma step_sextw: 
-  assumes decode_sextw: \<open>\<And>\<Delta> var. (\<Delta>, (address \<Colon> 64), var) \<mapsto>\<^sub>b\<^sub>i\<^sub>l \<lparr> addr = (address \<Colon> 64), size = (4 \<Colon> 64), code = [rd := extend:64[low:32[(rs1 :\<^sub>t imm\<langle>64\<rangle>)]]]\<rparr>\<close>
+  assumes decode_sextw: \<open>\<And>\<Delta> var. (\<Delta>, w, var) \<mapsto>\<^sub>b\<^sub>i\<^sub>l sextw w rd rs1\<close>
       and \<open>(rs1 :\<^sub>t imm\<langle>64\<rangle>, val \<Colon> 64) \<in>\<^sub>\<Delta> \<Delta>\<close>
-    shows \<open>(\<Delta>, address \<Colon> 64, var) \<leadsto>\<^sub>b\<^sub>i\<^sub>l (\<Delta>(rd \<mapsto> (ext (ext val \<Colon> 64 \<sim> hi : 32 - 1 \<sim> lo : 0) \<sim> hi : 64 - 1 \<sim> lo : 0)), (address \<Colon> 64) +\<^sub>b\<^sub>v (4 \<Colon> 64), var)\<close>
+    shows \<open>(\<Delta>, w, var) \<leadsto>\<^sub>b\<^sub>i\<^sub>l (\<Delta>(rd \<mapsto> (ext (ext val \<Colon> 64 \<sim> hi : 32 - 1 \<sim> lo : 0) \<sim> hi : 64 - 1 \<sim> lo : 0)), (w) +\<^sub>b\<^sub>v (4 \<Colon> 64), var)\<close>
   apply (insert assms(2-))
   by (solve_progI decoder: decode_sextw)
 
 subsubsection \<open>SD\<close>
 
+abbreviation \<open>sd w rs1 imm rs2 \<equiv> \<lparr> addr = w, size = (2 \<Colon> 64), code = [mem := (mem with [(rs1 :\<^sub>t imm\<langle>64\<rangle>) + (imm \<Colon> 64), el]:u64 \<leftarrow> (rs2 :\<^sub>t imm\<langle>64\<rangle>))] \<rparr>\<close>
+
 lemma step_sd:
-  assumes decode_sd: \<open>\<And>\<Delta> var. (\<Delta>, (address \<Colon> 64), var) \<mapsto>\<^sub>b\<^sub>i\<^sub>l \<lparr> addr = (address \<Colon> 64), size = (2 \<Colon> 64), code = [mem := (mem with [(rs1 :\<^sub>t imm\<langle>64\<rangle>) + (imm \<Colon> 64), el]:u64 \<leftarrow> (rs2 :\<^sub>t imm\<langle>64\<rangle>))]\<rparr>\<close>
+  assumes decode_sd: \<open>\<And>\<Delta> var. (\<Delta>, (w), var) \<mapsto>\<^sub>b\<^sub>i\<^sub>l sd w rs1 imm rs2\<close>
       and \<open>((rs1 :\<^sub>t imm\<langle>64\<rangle>), mem_addr \<Colon> 64) \<in>\<^sub>\<Delta> \<Delta>\<close> and \<open>((rs2 :\<^sub>t imm\<langle>64\<rangle>), val \<Colon> 64) \<in>\<^sub>\<Delta> \<Delta>\<close> and \<open>(mem, mem') \<in>\<^sub>\<Delta> \<Delta>\<close> and \<open>type mem' = mem\<langle>64, 8\<rangle>\<close>
-    shows \<open>(\<Delta>, (address \<Colon> 64), var) \<leadsto>\<^sub>b\<^sub>i\<^sub>l (\<Delta>(mem \<mapsto> storage_el64 mem' ((mem_addr \<Colon> 64) +\<^sub>b\<^sub>v (imm \<Colon> 64)) (val \<Colon> 64)), (address \<Colon> 64) +\<^sub>b\<^sub>v (2 \<Colon> 64), var)\<close>
+    shows \<open>(\<Delta>, (w), var) \<leadsto>\<^sub>b\<^sub>i\<^sub>l (\<Delta>(mem \<mapsto> storage_el64 mem' ((mem_addr \<Colon> 64) +\<^sub>b\<^sub>v (imm \<Colon> 64)) (val \<Colon> 64)), (w) +\<^sub>b\<^sub>v (2 \<Colon> 64), var)\<close>
   apply (insert assms(2-))
   apply (solve_progI decoder: decode_sd)
   unfolding Val_simp_storage
@@ -50,73 +56,88 @@ lemma step_sd:
 
 subsection \<open>AUIPC\<close>
 
+abbreviation \<open>auipc w rd imm \<equiv> \<lparr> addr = w, size = (4 \<Colon> 64), code = [rd := (imm \<Colon> 64)] \<rparr>\<close>
+
 lemma step_auipc:
-  assumes decode_auipc: \<open>\<And>\<Delta> var. (\<Delta>, address \<Colon> 64, var) \<mapsto>\<^sub>b\<^sub>i\<^sub>l \<lparr> addr = (address \<Colon> 64), size = (4 \<Colon> 64), code = [rd := (imm \<Colon> 64)]\<rparr>\<close>
-    shows \<open>(\<Delta>, address \<Colon> 64, var) \<leadsto>\<^sub>b\<^sub>i\<^sub>l (\<Delta>(rd \<mapsto> imm \<Colon> 64), (address \<Colon> 64) +\<^sub>b\<^sub>v (4 \<Colon> 64), var)\<close>
+  assumes decode_auipc: \<open>\<And>\<Delta> var. (\<Delta>, w, var) \<mapsto>\<^sub>b\<^sub>i\<^sub>l auipc w rd imm\<close>
+    shows \<open>(\<Delta>, w, var) \<leadsto>\<^sub>b\<^sub>i\<^sub>l (\<Delta>(rd \<mapsto> imm \<Colon> 64), (w) +\<^sub>b\<^sub>v (4 \<Colon> 64), var)\<close>
   apply (insert assms)
   by (solve_progI decoder: decode_auipc)
 
 subsubsection \<open>LI\<close>
 
+abbreviation \<open>li w rd imm \<equiv> \<lparr> addr = w, size = (2 \<Colon> 64), code = [rd := (imm \<Colon> 64)] \<rparr>\<close>
+
 lemma step_li:
-  assumes decode_li: \<open>\<And>\<Delta> var. (\<Delta>, address \<Colon> 64, var) \<mapsto>\<^sub>b\<^sub>i\<^sub>l \<lparr> addr = (address \<Colon> 64), size = (2 \<Colon> 64), code = [rd := (imm \<Colon> 64)]\<rparr>\<close>
-    shows \<open>(\<Delta>, address \<Colon> 64, var) \<leadsto>\<^sub>b\<^sub>i\<^sub>l (\<Delta>(rd \<mapsto> imm \<Colon> 64), (address \<Colon> 64) +\<^sub>b\<^sub>v (2 \<Colon> 64), var)\<close>
+  assumes decode_li: \<open>\<And>\<Delta> var. (\<Delta>, w, var) \<mapsto>\<^sub>b\<^sub>i\<^sub>l li w rd imm\<close>
+    shows \<open>(\<Delta>, w, var) \<leadsto>\<^sub>b\<^sub>i\<^sub>l (\<Delta>(rd \<mapsto> imm \<Colon> 64), (w) +\<^sub>b\<^sub>v (2 \<Colon> 64), var)\<close>
   apply (insert assms)
   by (solve_progI decoder: decode_li)
 
 subsubsection \<open>JAL\<close>
 
+abbreviation \<open>jal w ret target \<equiv> \<lparr> addr = w, size = (4 \<Colon> 64), code = [X1 := (ret \<Colon> 64), jmp (target \<Colon> 64)]\<rparr>\<close>
+
 lemma step_jal: 
-  assumes decode_jal:  \<open>\<And>\<Delta> var. (\<Delta>, address \<Colon> 64, var) \<mapsto>\<^sub>b\<^sub>i\<^sub>l \<lparr> addr = (address \<Colon> 64), size = (4 \<Colon> 64), code = [X1 := (ret \<Colon> 64), jmp (target \<Colon> 64)]\<rparr>\<close>
-    shows \<open>(\<Delta>, (address \<Colon> 64), var) \<leadsto>\<^sub>b\<^sub>i\<^sub>l (\<Delta>(X1 \<mapsto> (ret \<Colon> 64)), (target \<Colon> 64), var)\<close>
+  assumes decode_jal:  \<open>\<And>\<Delta> var. (\<Delta>, w, var) \<mapsto>\<^sub>b\<^sub>i\<^sub>l jal w ret target\<close>
+    shows \<open>(\<Delta>, (w), var) \<leadsto>\<^sub>b\<^sub>i\<^sub>l (\<Delta>(X1 \<mapsto> (ret \<Colon> 64)), (target \<Colon> 64), var)\<close>
   by (solve_progI decoder: decode_jal)
 
 subsubsection \<open>JALR\<close>
- 
-lemma step_jalr: 
-  assumes decode_jalr:  \<open>\<And>\<Delta> var. (\<Delta>, address \<Colon> 64, var) \<mapsto>\<^sub>b\<^sub>i\<^sub>l \<lparr> addr = (address \<Colon> 64), size = (4 \<Colon> 64), code = [X1 := (ret \<Colon> 64), jmp (target \<Colon> 64)]\<rparr>\<close>
-      and \<open>((rs1 :\<^sub>t imm\<langle>64\<rangle>), mem_addr \<Colon> 64) \<in>\<^sub>\<Delta> \<Delta>\<close> 
-    shows \<open>(\<Delta>, (address \<Colon> 64), var) \<leadsto>\<^sub>b\<^sub>i\<^sub>l (\<Delta>(X1 \<mapsto> (ret \<Colon> 64)), (target \<Colon> 64), var)\<close>
+
+abbreviation \<open>jalr w rs1 ret target \<equiv> \<lparr> addr = w, size = (4 \<Colon> 64), code = [X6 := (ret \<Colon> 64), jmp ((rs1 :\<^sub>t imm\<langle>64\<rangle>) + (target \<Colon> 64))]\<rparr>\<close>
+
+lemma step_jalr:
+  assumes decode_jalr:  \<open>\<And>\<Delta> var. (\<Delta>, w, var) \<mapsto>\<^sub>b\<^sub>i\<^sub>l jalr w rs1 ret target\<close>
+      and \<open>((rs1 :\<^sub>t imm\<langle>64\<rangle>), val \<Colon> 64) \<in>\<^sub>\<Delta> \<Delta>\<close> and \<open>X6 \<noteq> (rs1 :\<^sub>t imm\<langle>64\<rangle>)\<close>
+    shows \<open>(\<Delta>, (w), var) \<leadsto>\<^sub>b\<^sub>i\<^sub>l (\<Delta>(X6 \<mapsto> (ret \<Colon> 64)), ((val \<Colon> 64) +\<^sub>b\<^sub>v (target \<Colon> 64)), var)\<close>
+  using assms(2-) apply -
   by (solve_progI decoder: decode_jalr)
 
 subsubsection \<open>C.MV\<close>
 
 text \<open>Expansion of add rd, x0, rs2\<close>
 
+abbreviation \<open>mv w rd rs1 \<equiv> \<lparr> addr = w, size = (2 \<Colon> 64), code = [rd := (rs1 :\<^sub>t imm\<langle>64\<rangle>)]\<rparr>\<close>
+
 lemma step_mv: 
-  assumes decode_mv:  \<open>\<And>\<Delta> var. (\<Delta>, address \<Colon> 64, var) \<mapsto>\<^sub>b\<^sub>i\<^sub>l \<lparr> addr = (address \<Colon> 64), size = (2 \<Colon> 64), code = [rd := (rs1 :\<^sub>t imm\<langle>64\<rangle>)]\<rparr>\<close>
+  assumes decode_mv:  \<open>\<And>\<Delta> var. (\<Delta>, w, var) \<mapsto>\<^sub>b\<^sub>i\<^sub>l mv w rd rs1\<close>
       and \<open>((rs1 :\<^sub>t imm\<langle>64\<rangle>), val \<Colon> 64) \<in>\<^sub>\<Delta> \<Delta>\<close> 
-    shows \<open>(\<Delta>, (address \<Colon> 64), var) \<leadsto>\<^sub>b\<^sub>i\<^sub>l (\<Delta>(rd \<mapsto> (val \<Colon> 64)), (address \<Colon> 64) +\<^sub>b\<^sub>v (2 \<Colon> 64), var)\<close>
+    shows \<open>(\<Delta>, (w), var) \<leadsto>\<^sub>b\<^sub>i\<^sub>l (\<Delta>(rd \<mapsto> (val \<Colon> 64)), (w) +\<^sub>b\<^sub>v (2 \<Colon> 64), var)\<close>
   apply (insert assms(2-))
   by (solve_progI decoder: decode_mv)
 
 subsection \<open>LW\<close>
 
+abbreviation \<open>lw w rd rs1 imm \<equiv> \<lparr> addr = w, size = (4 \<Colon> 64), code = [(rd :\<^sub>t imm\<langle>64\<rangle>) := (extend:64[mem[(rs1 :\<^sub>t imm\<langle>64\<rangle>) + (imm \<Colon> 64), el]:u32])]\<rparr>\<close>
+
 lemma step_lw: 
-  assumes decode_lw:  \<open>\<And>\<Delta> var. (\<Delta>, address \<Colon> 64, var) \<mapsto>\<^sub>b\<^sub>i\<^sub>l \<lparr> addr = (address \<Colon> 64), size = (4 \<Colon> 64), code = [(rd :\<^sub>t imm\<langle>64\<rangle>) := extend:64[mem[(rs1 :\<^sub>t imm\<langle>64\<rangle>) + (imm \<Colon> 64), el]:u32]]\<rparr>\<close>
+  assumes decode_lw:  \<open>\<And>\<Delta> var. (\<Delta>, w, var) \<mapsto>\<^sub>b\<^sub>i\<^sub>l lw w rd rs1 imm\<close>
       and \<open>((rs1 :\<^sub>t imm\<langle>64\<rangle>), mem_addr \<Colon> 64) \<in>\<^sub>\<Delta> \<Delta>\<close> and \<open>(mem, mem') \<in>\<^sub>\<Delta> \<Delta>\<close>
       and load: \<open>\<And>\<Delta>. \<Delta> \<turnstile> extend:64[(Val mem')[(mem_addr \<Colon> 64) +\<^sub>b\<^sub>v (imm \<Colon> 64), el]:u32] \<leadsto>* (val \<Colon> 64)\<close>
-    shows \<open>(\<Delta>, (address \<Colon> 64), var) \<leadsto>\<^sub>b\<^sub>i\<^sub>l (\<Delta>((rd :\<^sub>t imm\<langle>64\<rangle>) \<mapsto> (val \<Colon> 64)), (address \<Colon> 64) +\<^sub>b\<^sub>v (4 \<Colon> 64), var)\<close>
+    shows \<open>(\<Delta>, (w), var) \<leadsto>\<^sub>b\<^sub>i\<^sub>l (\<Delta>((rd :\<^sub>t imm\<langle>64\<rangle>) \<mapsto> (val \<Colon> 64)), (w) +\<^sub>b\<^sub>v (4 \<Colon> 64), var)\<close>
   apply (insert assms(2-3))
   apply (solve_progI decoder: decode_lw)
   unfolding Val_simp_word by (rule load)
 
 subsection \<open>SW\<close>
 
+abbreviation \<open>sw w rs1 imm rs2 \<equiv> \<lparr> addr = w, size = (4 \<Colon> 64), code = [mem := (mem with [(rs1 :\<^sub>t imm\<langle>64\<rangle>) + (imm \<Colon> 64), el]:u32 \<leftarrow> (low:32[(rs2 :\<^sub>t imm\<langle>64\<rangle>)]))]\<rparr>\<close>
+
 lemma step_sw: 
-  assumes decode_sw:  \<open>\<And>\<Delta> var. (\<Delta>, address \<Colon> 64, var) \<mapsto>\<^sub>b\<^sub>i\<^sub>l \<lparr> addr = (address \<Colon> 64), size = (4 \<Colon> 64), code = [mem := mem with [(rs1 :\<^sub>t imm\<langle>64\<rangle>) + (imm \<Colon> 64), el]:u32 \<leftarrow> low:32[(rs2 :\<^sub>t imm\<langle>64\<rangle>)]]\<rparr>\<close>
+  assumes decode_sw:  \<open>\<And>\<Delta> var. (\<Delta>, w, var) \<mapsto>\<^sub>b\<^sub>i\<^sub>l sw w rs1 imm rs2\<close>
       and \<open>((rs1 :\<^sub>t imm\<langle>64\<rangle>), mem_addr \<Colon> 64) \<in>\<^sub>\<Delta> \<Delta>\<close> and \<open>((rs2 :\<^sub>t imm\<langle>64\<rangle>), val \<Colon> 64) \<in>\<^sub>\<Delta> \<Delta>\<close> and \<open>(mem, mem') \<in>\<^sub>\<Delta> \<Delta>\<close> and \<open>type mem' = mem\<langle>64, 8\<rangle>\<close>
-    shows \<open>(\<Delta>, (address \<Colon> 64), var) \<leadsto>\<^sub>b\<^sub>i\<^sub>l (\<Delta>(mem \<mapsto> storage32 mem' ((mem_addr + imm) mod 18446744073709551616) 64 (take_bit 32 val)), (address \<Colon> 64) +\<^sub>b\<^sub>v (4 \<Colon> 64), var)\<close>
+    shows \<open>(\<Delta>, (w), var) \<leadsto>\<^sub>b\<^sub>i\<^sub>l (\<Delta>(mem \<mapsto> storage32 mem' (((mem_addr + imm) mod 18446744073709551616) \<Colon> 64) ((take_bit 32 val) \<Colon> 64)), (w) +\<^sub>b\<^sub>v (4 \<Colon> 64), var)\<close>
   apply (insert assms(2-))
   apply (solve_progI decoder: decode_sw)
   oops (* store32 *)
 
-  subsection \<open>BEQZ\<close>
+subsection \<open>BEQZ\<close>
 
 lemma step_beqz:
-  assumes decode_beqz: \<open>\<And>\<Delta> var. (\<Delta>, address \<Colon> 64, var) \<mapsto>\<^sub>b\<^sub>i\<^sub>l \<lparr> addr = (address \<Colon> 64), size = (2 \<Colon> 64), code = [temp :\<^sub>t imm\<langle>1\<rangle> := BinOp (rs1 :\<^sub>t imm\<langle>64\<rangle>) (LOp Eq) (0 \<Colon> 64), IfThen (temp :\<^sub>t imm\<langle>1\<rangle>) [jmp (offset \<Colon> 64)]]\<rparr>\<close>
+  assumes decode_beqz: \<open>\<And>\<Delta> var. (\<Delta>, w, var) \<mapsto>\<^sub>b\<^sub>i\<^sub>l \<lparr> addr = (w), size = (2 \<Colon> 64), code = [temp :\<^sub>t imm\<langle>1\<rangle> := BinOp (rs1 :\<^sub>t imm\<langle>64\<rangle>) (LOp Eq) (0 \<Colon> 64), IfThen (temp :\<^sub>t imm\<langle>1\<rangle>) [jmp (offset \<Colon> 64)]]\<rparr>\<close>
       and \<open>((rs1 :\<^sub>t imm\<langle>64\<rangle>), cond \<Colon> 64) \<in>\<^sub>\<Delta> \<Delta>\<close>
-    shows \<open>(\<Delta>, (address \<Colon> 64), var) \<leadsto>\<^sub>b\<^sub>i\<^sub>l (\<Delta>((temp :\<^sub>t imm\<langle>1\<rangle>) \<mapsto> true), (offset \<Colon> 64), var) \<or> (\<Delta>, (address \<Colon> 64), var) \<leadsto>\<^sub>b\<^sub>i\<^sub>l (\<Delta>((temp :\<^sub>t imm\<langle>1\<rangle>) \<mapsto> false), (address \<Colon> 64) +\<^sub>b\<^sub>v (2 \<Colon> 64), var)\<close>
+    shows \<open>(\<Delta>, (w), var) \<leadsto>\<^sub>b\<^sub>i\<^sub>l (\<Delta>((temp :\<^sub>t imm\<langle>1\<rangle>) \<mapsto> true), (offset \<Colon> 64), var) \<or> (\<Delta>, (w), var) \<leadsto>\<^sub>b\<^sub>i\<^sub>l (\<Delta>((temp :\<^sub>t imm\<langle>1\<rangle>) \<mapsto> false), (w) +\<^sub>b\<^sub>v (2 \<Colon> 64), var)\<close>
 proof (cases \<open>cond = 0\<close>)
   case True
   show ?thesis 
@@ -133,10 +154,10 @@ qed
 subsection \<open>LD\<close>
 
 lemma step_ld:
-  assumes decode_ld: \<open>\<And>\<Delta> var. (\<Delta>, address \<Colon> 64, var) \<mapsto>\<^sub>b\<^sub>i\<^sub>l \<lparr> addr = (address \<Colon> 64), size = (4 \<Colon> 64), code = [rd := (mem[(rs1 :\<^sub>t imm\<langle>64\<rangle>) + (imm \<Colon> 64), el]:u64)]\<rparr>\<close>
+  assumes decode_ld: \<open>\<And>\<Delta> var. (\<Delta>, w, var) \<mapsto>\<^sub>b\<^sub>i\<^sub>l \<lparr> addr = (w), size = (4 \<Colon> 64), code = [rd := (mem[(rs1 :\<^sub>t imm\<langle>64\<rangle>) + (imm \<Colon> 64), el]:u64)]\<rparr>\<close>
       and \<open>((rs1 :\<^sub>t imm\<langle>64\<rangle>), (mem_addr \<Colon> 64)) \<in>\<^sub>\<Delta> \<Delta>\<close> and \<open>(mem, mem') \<in>\<^sub>\<Delta> \<Delta>\<close>
       and load: \<open>\<Delta> \<turnstile> (Val mem')[(mem_addr \<Colon> 64) +\<^sub>b\<^sub>v (imm \<Colon> 64), el]:u64 \<leadsto>* (ptr \<Colon> 64)\<close>
-    shows \<open>(\<Delta>, (address \<Colon> 64), var) \<leadsto>\<^sub>b\<^sub>i\<^sub>l (\<Delta>(rd \<mapsto> ptr \<Colon> 64), (address \<Colon> 64) +\<^sub>b\<^sub>v (4 \<Colon> 64), var)\<close>
+    shows \<open>(\<Delta>, (w), var) \<leadsto>\<^sub>b\<^sub>i\<^sub>l (\<Delta>(rd \<mapsto> ptr \<Colon> 64), (w) +\<^sub>b\<^sub>v (4 \<Colon> 64), var)\<close>
   apply (insert assms(2-3))
   apply (solve_progI decoder: decode_ld)
   unfolding Val_simp_word by (rule load)
@@ -144,10 +165,10 @@ lemma step_ld:
 subsection \<open>C.LD\<close>
 
 lemma step_cld:
-  assumes decode_cld: \<open>\<And>\<Delta> var. (\<Delta>, address \<Colon> 64, var) \<mapsto>\<^sub>b\<^sub>i\<^sub>l \<lparr> addr = (address \<Colon> 64), size = (2 \<Colon> 64), code = [rd := (mem[(rs1 :\<^sub>t imm\<langle>64\<rangle>) + (imm \<Colon> 64), el]:u64)]\<rparr>\<close>
+  assumes decode_cld: \<open>\<And>\<Delta> var. (\<Delta>, w, var) \<mapsto>\<^sub>b\<^sub>i\<^sub>l \<lparr> addr = (w), size = (2 \<Colon> 64), code = [rd := (mem[(rs1 :\<^sub>t imm\<langle>64\<rangle>) + (imm \<Colon> 64), el]:u64)]\<rparr>\<close>
       and \<open>((rs1 :\<^sub>t imm\<langle>64\<rangle>), (mem_addr \<Colon> 64)) \<in>\<^sub>\<Delta> \<Delta>\<close> and \<open>(mem, mem') \<in>\<^sub>\<Delta> \<Delta>\<close>
       and load: \<open>\<Delta> \<turnstile> (Val mem')[(mem_addr \<Colon> 64) +\<^sub>b\<^sub>v (imm \<Colon> 64), el]:u64 \<leadsto>* (ptr \<Colon> 64)\<close>
-    shows \<open>(\<Delta>, (address \<Colon> 64), var) \<leadsto>\<^sub>b\<^sub>i\<^sub>l (\<Delta>(rd \<mapsto> ptr \<Colon> 64), (address \<Colon> 64) +\<^sub>b\<^sub>v (2 \<Colon> 64), var)\<close>
+    shows \<open>(\<Delta>, (w), var) \<leadsto>\<^sub>b\<^sub>i\<^sub>l (\<Delta>(rd \<mapsto> ptr \<Colon> 64), (w) +\<^sub>b\<^sub>v (2 \<Colon> 64), var)\<close>
   apply (insert assms(2-3))
   apply (solve_progI decoder: decode_cld)
   unfolding Val_simp_word by (rule load)
@@ -155,40 +176,39 @@ lemma step_cld:
 subsection \<open>J\<close>
 
 lemma step_j:
-  assumes decode_j: \<open>\<And>\<Delta> var. (\<Delta>, address \<Colon> 64, var) \<mapsto>\<^sub>b\<^sub>i\<^sub>l \<lparr> addr = (address \<Colon> 64), size = (2 \<Colon> 64), code = [jmp (offset \<Colon> 64)]\<rparr>\<close>
-    shows \<open>(\<Delta>, (address \<Colon> 64), var) \<leadsto>\<^sub>b\<^sub>i\<^sub>l (\<Delta>, (offset \<Colon> 64), var)\<close>
+  assumes decode_j: \<open>\<And>\<Delta> var. (\<Delta>, w, var) \<mapsto>\<^sub>b\<^sub>i\<^sub>l \<lparr> addr = (w), size = (2 \<Colon> 64), code = [jmp (offset \<Colon> 64)]\<rparr>\<close>
+    shows \<open>(\<Delta>, (w), var) \<leadsto>\<^sub>b\<^sub>i\<^sub>l (\<Delta>, (offset \<Colon> 64), var)\<close>
   by (solve_progI decoder: decode_j)
 
 subsection \<open>NOP\<close>
 
 lemma step_nop:
-  assumes decode_nop: \<open>\<And>\<Delta> var. (\<Delta>, address \<Colon> 64, var) \<mapsto>\<^sub>b\<^sub>i\<^sub>l \<lparr> addr = (address \<Colon> 64), size = (2 \<Colon> 64), code = []\<rparr>\<close>
-    shows \<open>(\<Delta>, (address \<Colon> 64), var) \<leadsto>\<^sub>b\<^sub>i\<^sub>l (\<Delta>, (address \<Colon> 64) +\<^sub>b\<^sub>v (2 \<Colon> 64), var)\<close>
+  assumes decode_nop: \<open>\<And>\<Delta> var. (\<Delta>, w, var) \<mapsto>\<^sub>b\<^sub>i\<^sub>l \<lparr> addr = (w), size = (2 \<Colon> 64), code = []\<rparr>\<close>
+    shows \<open>(\<Delta>, (w), var) \<leadsto>\<^sub>b\<^sub>i\<^sub>l (\<Delta>, (w) +\<^sub>b\<^sub>v (2 \<Colon> 64), var)\<close>
   by (solve_progI decoder: decode_nop)
 
 subsection \<open>LUI\<close>
 
 lemma step_lui:
-  assumes decode_lui: \<open>\<And>\<Delta> var. (\<Delta>, address \<Colon> 64, var) \<mapsto>\<^sub>b\<^sub>i\<^sub>l \<lparr> addr = (address \<Colon> 64), size = (2 \<Colon> 64), code = [rd := (imm \<Colon> 64)]\<rparr>\<close>
-    shows \<open>(\<Delta>, (address \<Colon> 64), var) \<leadsto>\<^sub>b\<^sub>i\<^sub>l (\<Delta>(rd \<mapsto> (imm \<Colon> 64)), (address \<Colon> 64) +\<^sub>b\<^sub>v (2 \<Colon> 64), var)\<close>
+  assumes decode_lui: \<open>\<And>\<Delta> var. (\<Delta>, w, var) \<mapsto>\<^sub>b\<^sub>i\<^sub>l \<lparr> addr = (w), size = (2 \<Colon> 64), code = [rd := (imm \<Colon> 64)]\<rparr>\<close>
+    shows \<open>(\<Delta>, (w), var) \<leadsto>\<^sub>b\<^sub>i\<^sub>l (\<Delta>(rd \<mapsto> (imm \<Colon> 64)), (w) +\<^sub>b\<^sub>v (2 \<Colon> 64), var)\<close>
   by (solve_progI decoder: decode_lui)
 
 subsection \<open>BGE\<close>
 
 (* address + offset *)
 lemma step_bge_true:
-  assumes decode_bge: \<open>\<And>\<Delta> var. (\<Delta>, address \<Colon> 64, var) \<mapsto>\<^sub>b\<^sub>i\<^sub>l \<lparr> addr = (address \<Colon> 64), size = (4 \<Colon> 64), code = [(ivar :\<^sub>t imm\<langle>1\<rangle>) := (rs1 :\<^sub>t imm\<langle>64\<rangle>) le (rs2 :\<^sub>t imm\<langle>64\<rangle>), IfThen (ivar :\<^sub>t imm\<langle>1\<rangle>) [jmp (offset \<Colon> 64)]]\<rparr>\<close>
+  assumes decode_bge: \<open>\<And>\<Delta> var. (\<Delta>, w, var) \<mapsto>\<^sub>b\<^sub>i\<^sub>l \<lparr> addr = (w), size = (4 \<Colon> 64), code = [(ivar :\<^sub>t imm\<langle>1\<rangle>) := (rs1 :\<^sub>t imm\<langle>64\<rangle>) le (rs2 :\<^sub>t imm\<langle>64\<rangle>), IfThen (ivar :\<^sub>t imm\<langle>1\<rangle>) [jmp (offset \<Colon> 64)]]\<rparr>\<close>
       and \<open>((rs1 :\<^sub>t imm\<langle>64\<rangle>), num1 \<Colon> 64) \<in>\<^sub>\<Delta> \<Delta>\<close> and \<open>((rs2 :\<^sub>t imm\<langle>64\<rangle>), num2 \<Colon> 64) \<in>\<^sub>\<Delta> \<Delta>\<close>
       and leq: \<open>(num1 \<Colon> 64) \<le>\<^sub>b\<^sub>v (num2 \<Colon> 64) = (true::val)\<close>
-    shows \<open>(\<Delta>, (address \<Colon> 64), var) \<leadsto>\<^sub>b\<^sub>i\<^sub>l (\<Delta>(ivar :\<^sub>t imm\<langle>1\<rangle> \<mapsto> true), (offset \<Colon> 64), var)\<close>
-  apply (insert assms(2-3), solve_progI decoder: decode_bge)
-  unfolding leq by solve_bilI
+    shows \<open>(\<Delta>, (w), var) \<leadsto>\<^sub>b\<^sub>i\<^sub>l (\<Delta>(ivar :\<^sub>t imm\<langle>1\<rangle> \<mapsto> true), (offset \<Colon> 64), var)\<close>
+  by (insert assms(2-3), solve_prog_intI assumption simp: leq decoder: decode_bge)
 
 lemma step_bge_false:
-  assumes decode_bge: \<open>\<And>\<Delta> var. (\<Delta>, address \<Colon> 64, var) \<mapsto>\<^sub>b\<^sub>i\<^sub>l \<lparr> addr = (address \<Colon> 64), size = (4 \<Colon> 64), code = [(ivar :\<^sub>t imm\<langle>1\<rangle>) := (rs1 :\<^sub>t imm\<langle>64\<rangle>) le (rs2 :\<^sub>t imm\<langle>64\<rangle>), IfThen (ivar :\<^sub>t imm\<langle>1\<rangle>) [jmp (offset \<Colon> 64)]]\<rparr>\<close>
+  assumes decode_bge: \<open>\<And>\<Delta> var. (\<Delta>, w, var) \<mapsto>\<^sub>b\<^sub>i\<^sub>l \<lparr> addr = (w), size = (4 \<Colon> 64), code = [(ivar :\<^sub>t imm\<langle>1\<rangle>) := (rs1 :\<^sub>t imm\<langle>64\<rangle>) le (rs2 :\<^sub>t imm\<langle>64\<rangle>), IfThen (ivar :\<^sub>t imm\<langle>1\<rangle>) [jmp (offset \<Colon> 64)]]\<rparr>\<close>
       and \<open>((rs1 :\<^sub>t imm\<langle>64\<rangle>), num1 \<Colon> 64) \<in>\<^sub>\<Delta> \<Delta>\<close> and \<open>((rs2 :\<^sub>t imm\<langle>64\<rangle>), num2 \<Colon> 64) \<in>\<^sub>\<Delta> \<Delta>\<close>
       and \<open>(num1 \<Colon> 64) \<le>\<^sub>b\<^sub>v (num2 \<Colon> 64) = (false::val)\<close>
-    shows \<open>(\<Delta>, (address \<Colon> 64), var) \<leadsto>\<^sub>b\<^sub>i\<^sub>l (\<Delta>(ivar :\<^sub>t imm\<langle>1\<rangle> \<mapsto> false), (address \<Colon> 64) +\<^sub>b\<^sub>v (4 \<Colon> 64), var)\<close>
+    shows \<open>(\<Delta>, (w), var) \<leadsto>\<^sub>b\<^sub>i\<^sub>l (\<Delta>(ivar :\<^sub>t imm\<langle>1\<rangle> \<mapsto> false), (w) +\<^sub>b\<^sub>v (4 \<Colon> 64), var)\<close>
   by (insert assms(2-), solve_progI decoder: decode_bge)
 
 
@@ -200,6 +220,7 @@ method solve_riscvI uses decoder = (
   | (rule step_lw, rule decoder, (solve_in_var, solve_in_var)?)
   | (rule step_mv, rule decoder, solve_in_var?)
   | (rule step_jal, rule decoder)
+  | (rule step_jalr, rule decoder, solve_in_var?, simp (no_asm))
   | (rule step_auipc, rule decoder) \<comment> \<open>step_li\<close>
   | (rule step_sd, rule decoder, (solve_in_var, solve_in_var, solve_in_var)?)
   | (rule step_addi, rule decoder, solve_in_var?)
